***NO_CI*** Standard heap on top of monotonic heap.

ulib/FStar.Heap.fst
@@ -3,95 +3,65 @@ module FStar.Heap
 open FStar.Classical
 open FStar.Set
 
+open FStar.Monotonic.Heap
+
 (* Heap is a tuple of a source of freshness (the no. of the next 
    reference to be allocated) and a mapping of allocated raw 
    references (represented as natural numbers) to types and values. *)
 
-abstract noeq type heap_rec = {
-  next_addr: nat;
-  memory   : nat -> Tot (option (a:Type0 & a))
-}  
-abstract type heap = h:heap_rec{(forall (n:nat). n >= h.next_addr ==> None? (h.memory n))}
+abstract let heap = heap
 
-(* Consistency of heaps. aka, no strong updates *)
-private let consistent (h0:heap) (h1:heap)
-  = forall n x y. (h0.memory n == Some x /\ h1.memory n == Some y) ==> dfst x == dfst y
+abstract let ref (a:Type0) = mref a (fun _ _ -> True)
 
-(* References: address * initial value * manually managed flag *)
-abstract noeq type ref (a:Type0) = {
-  addr: nat;
-  init: a;
-  mm:   bool;  //manually managed flag
-}  
+//private let as_mref (#a:Type0) (r:ref a) :Tot (mref a (fun _ _ -> True)) = r
 
-abstract let addr_of (#a:Type) (r:ref a) :GTot nat = r.addr
+abstract let addr_of (#a:Type) (r:ref a) :GTot nat = addr_of r
 
-abstract let is_mm (#a:Type) (r:ref a) :GTot bool = r.mm
+abstract let is_mm (#a:Type) (r:ref a) :GTot bool = is_mm r
 
 abstract let compare_addrs (#a:Type) (#b:Type) (r1:ref a) (r2:ref b)
   :(b:bool{b = (addr_of r1 = addr_of r2)})
-  = r1.addr = r2.addr
+  = compare_addrs r1 r2
 
-abstract let contains (#a:Type0) (h:heap) (r:ref a)
-  = Some? (h.memory r.addr) /\ dfst (Some?.v (h.memory r.addr)) == a
+abstract val contains: #a:Type0 -> heap -> ref a -> GTot Type0
+let contains #a h r = contains h r 
 
-abstract let unused_in (#a:Type) (r:ref a) (h:heap) :Type0
-  = None? (h.memory r.addr)
+abstract val unused_in: #a:Type0 -> ref a -> heap -> GTot Type0
+let unused_in #a r h = unused_in r h
 
-let fresh (#a:Type) (r:ref a) (h0:heap) (h1:heap) =
-  r `unused_in` h0 /\ h1 `contains` r
+val fresh: #a:Type0 -> ref a -> heap -> heap -> GTot Type0
+let fresh #a r h0 h1 = fresh r h0 h1
 
 let only x = singleton (addr_of x)
 
 (* Select. *)
 private abstract let sel_tot (#a:Type) (h:heap) (r:ref a{h `contains` r}) :a
-  = let Some (| _, x |) = h.memory r.addr in
-    x
+  = sel_tot h r
 
 abstract let sel (#a:Type) (h:heap) (r:ref a) :GTot a
-  = if FStar.StrongExcludedMiddle.strong_excluded_middle (h `contains` r) then
-      sel_tot #a h r
-    else r.init
+  = sel h r
+
 
 (* Update. *)
 abstract let upd_tot (#a:Type) (h:heap) (r:ref a{h `contains` r}) (x:a) :heap
-  = { h with memory = (fun r' -> if r.addr = r'
-			      then Some (| a, x |)
-                              else h.memory r') }
+  = upd_tot h r x
 
 abstract let upd (#a:Type) (h:heap) (r:ref a) (x:a) :GTot heap
-  = if FStar.StrongExcludedMiddle.strong_excluded_middle (h `contains` r)
-    then upd_tot h r x
-    else
-      if r.addr >= h.next_addr
-      then (* alloc at r.addr *)
-        { next_addr = r.addr + 1;
-          memory    = (fun (r':nat) -> if r' = r.addr
-	   		           then Some (| a, x |)
-                                   else h.memory r') }
-      else (* strong update at r.addr *)
-        { h with memory = (fun r' -> if r' = r.addr
-				  then Some (| a, x |)
-                                  else h.memory r') }
+  = upd h r x
 
 (* Allocate. *)
 abstract let alloc (#a:Type) (h:heap) (x:a) (mm:bool) :GTot (ref a * heap)
-  = let r = { addr = h.next_addr; init = x; mm = mm } in
-    r, upd #a h r x
-
+  = alloc h x (fun _ _ -> True) mm
+  
 abstract let free_mm (#a:Type) (h:heap) (r:ref a{h `contains` r /\ is_mm r})
   :GTot heap
-  = { h with memory = (fun r' -> if r' = r.addr then None else h.memory r') }
+  = free_mm h r
 
-let modifies (s:set nat) (h0:heap) (h1:heap) =
-  (forall (a:Type) (r:ref a).{:pattern (sel h1 r)}
-                         ((~ (mem (addr_of r) s)) /\ h0 `contains` r) ==> sel h1 r == sel h0 r) /\
-  (forall (a:Type) (r:ref a).{:pattern (contains h1 r)}
-                        h0 `contains` r ==> h1 `contains` r) /\
-  (forall (a:Type) (r:ref a).{:pattern (r `unused_in` h0)}
-                        r `unused_in` h1 ==> r `unused_in` h0)
+val modifies: s:set nat -> heap -> heap -> GTot Type0
+let modifies s h0 h1 = modifies s h0 h1
 
 (** some lemmas that summarize the behavior **)
+
 
 (*
  * update of a well-typed reference
@@ -118,7 +88,7 @@ private let lemma_upd_contains_not_necessarily_well_typed_test
           (let h1 = upd h0 r x in
 	   h1 `contains` r /\
            (forall (b:Type) (r':ref b). addr_of r' <> addr_of r ==> sel h0 r' == sel h1 r')           /\
-	   (forall (b:Type) (r':ref b). (r'.addr <> r.addr /\ h0 `contains` r') ==> h1 `contains` r') /\
+	   (forall (b:Type) (r':ref b). (addr_of r' <> addr_of r /\ h0 `contains` r') ==> h1 `contains` r') /\
 	   (forall (b:Type) (r':ref b). r' `unused_in` h0 <==> r' `unused_in` h1)))
   = ()
 
@@ -169,41 +139,41 @@ let lemma_contains_implies_used
   :Lemma (requires (h `contains` r))
          (ensures  (~ (r `unused_in` h)))
 	 [SMTPatOr [[SMTPat (h `contains` r)]; [SMTPat (r `unused_in` h)]]]
-  = ()
+  = lemma_contains_implies_used h r
 
 let lemma_distinct_addrs_distinct_types
   (#a:Type) (#b:Type) (h:heap) (r1:ref a) (r2:ref b)
   :Lemma (requires (a =!= b /\ h `contains` r1 /\ h `contains` r2))
          (ensures  (addr_of r1 <> addr_of r2))
 	 [SMTPatT (h `contains` r1); SMTPatT (h `contains` r2)]
-  = ()
+  = lemma_distinct_addrs_distinct_types h r1 r2
 
 let lemma_distinct_addrs_unused
   (#a:Type) (#b:Type) (h:heap) (r1:ref a) (r2:ref b)
   :Lemma (requires (r1 `unused_in` h /\ ~ (r2 `unused_in` h)))
          (ensures  (addr_of r1 <> addr_of r2))
          [SMTPat (r1 `unused_in` h); SMTPat (r2 `unused_in` h)]
-  = ()
+  = lemma_distinct_addrs_unused h r1 r2
 
 let lemma_alloc (#a:Type) (h0:heap) (x:a) (mm:bool)
   :Lemma (requires True)
          (ensures  (let r, h1 = alloc h0 x mm in
                     h1 == upd h0 r x /\ fresh r h0 h1 /\ is_mm r = mm))
 	 [SMTPat (alloc h0 x mm)]
-  = ()
+  = lemma_alloc #a #(fun _ _ -> True) h0 x mm
 
 let lemma_free_mm_sel (#a:Type) (#b:Type) (h0:heap) (r:ref a{h0 `contains` r /\ is_mm r}) (r':ref b)
   :Lemma (requires True)
          (ensures  (addr_of r' <> addr_of r ==> sel h0 r' == sel (free_mm h0 r) r'))
 	 [SMTPat (sel (free_mm h0 r) r')]
-  = ()
+  = lemma_free_mm_sel h0 r r'
 
 let lemma_free_mm_contains (#a:Type) (#b:Type) (h0:heap) (r:ref a{h0 `contains` r /\ is_mm r}) (r':ref b)
   :Lemma (requires True)
          (ensures  (let h1 = free_mm h0 r in
 	            (addr_of r' <> addr_of r /\ h0 `contains` r') <==> h1 `contains` r'))
 	 [SMTPat ((free_mm h0 r) `contains` r')]
-  = ()
+  = lemma_free_mm_contains h0 r r'
 
 let lemma_free_mm_unused (#a:Type) (#b:Type) (h0:heap) (r:ref a{h0 `contains` r /\ is_mm r}) (r':ref b)
   :Lemma (requires True)
@@ -212,60 +182,60 @@ let lemma_free_mm_unused (#a:Type) (#b:Type) (h0:heap) (r:ref a{h0 `contains` r 
 		     (r' `unused_in` h0      ==> r' `unused_in` h1)      /\
 		     (r' `unused_in` h1      ==> (r' `unused_in` h0 \/ addr_of r' = addr_of r)))))
 	 [SMTPat (r' `unused_in` (free_mm h0 r))]
-  = ()
+  = lemma_free_mm_unused_m h0 r r'
 
 let lemma_sel_same_addr (#a:Type) (h:heap) (r1:ref a) (r2:ref a)
   :Lemma (requires (h `contains` r1 /\ addr_of r1 = addr_of r2))
          (ensures  (h `contains` r2 /\ sel h r1 == sel h r2))
 	 [SMTPat (sel h r1); SMTPat (sel h r2)]
-  = ()
+  = lemma_sel_same_addr h r1 r2
 
 let lemma_sel_upd1 (#a:Type) (h:heap) (r:ref a) (x:a) (r':ref a)
   :Lemma (requires (addr_of r = addr_of r'))
          (ensures  (sel (upd h r x) r' == x))
          [SMTPat (sel (upd h r x) r')]
 
-  = ()
+  = lemma_sel_upd1 h r x r'
 
 let lemma_sel_upd2 (#a:Type) (#b:Type) (h:heap) (r1:ref a) (r2:ref b) (x:b)
   :Lemma (requires (addr_of r1 <> addr_of r2))
          (ensures  (sel (upd h r2 x) r1 == sel h r1))
 	 [SMTPat (sel (upd h r2 x) r1)]
-  = ()
+  = lemma_sel_upd2 h r1 r2 x
 
 let lemma_ref_injectivity
   :(u:unit{forall (a:Type) (b:Type) (r1:ref a) (r2:ref b). a =!= b ==> ~ (eq3 r1 r2)})
-  = ()
+  = lemma_ref_injectivity
 
-
-let equal_dom (h1:heap) (h2:heap) :GTot Type0 =
-  (forall (a:Type0) (r:ref a). h1 `contains` r <==> h2 `contains` r) /\
-  (forall (a:Type0) (r:ref a). r `unused_in` h1 <==> r `unused_in` h2)
+let equal_dom (h1:heap) (h2:heap) :GTot Type0 = equal_dom h1 h2
+//  forall (a:Type0) (r:ref a). r `unused_in` h1 <==> r `unused_in` h2
 
 (* Empty. *)
-let emp :heap = {
+let emp :heap = emp
+
+(*let emp :heap = {
   next_addr = 0;
   memory    = (fun (r:nat) -> None)
-}
+}*)
 
 let lemma_in_dom_emp (#a:Type) (r:ref a)
   :Lemma (requires True)
          (ensures  (r `unused_in` emp))
 	 [SMTPat (r `unused_in` emp)]
-  = ()
+  = lemma_in_dom_emp r
 
 let lemma_upd_contains (#a:Type) (h:heap) (r:ref a) (x:a)
   :Lemma (requires True)
          (ensures  ((upd h r x) `contains` r))
 	 [SMTPat ((upd h r x) `contains` r)]
-  = ()
+  = lemma_upd_contains h r x
 
 let lemma_well_typed_upd_contains (#a:Type) (#b:Type) (h:heap) (r:ref a) (x:a) (r':ref b)
   :Lemma (requires (h `contains` r))
          (ensures  (let h1 = upd h r x in
 	            h1 `contains` r' <==> h `contains` r'))
 	 [SMTPat ((upd h r x) `contains` r')]
-  = ()
+  = lemma_well_typed_upd_contains h r x r'
 
 let lemma_unused_upd_contains (#a:Type) (#b:Type) (h:heap) (r:ref a) (x:a) (r':ref b)
   :Lemma (requires (r `unused_in` h))
@@ -273,13 +243,14 @@ let lemma_unused_upd_contains (#a:Type) (#b:Type) (h:heap) (r:ref a) (x:a) (r':r
 	            (h `contains` r'  ==> h1 `contains` r') /\
 		    (h1 `contains` r' ==> (h `contains` r' \/ addr_of r' = addr_of r))))
 	 [SMTPat ((upd h r x) `contains` r')]
-  = ()
+  = lemma_unused_upd_contains h r x r'
 
 let lemma_upd_contains_different_addr (#a:Type) (#b:Type) (h:heap) (r:ref a) (x:a) (r':ref b)
   :Lemma (requires (h `contains` r' /\ addr_of r <> addr_of r'))
          (ensures  ((upd h r x) `contains` r'))
 	 [SMTPat ((upd h r x) `contains` r')]
-  = ()
+  = lemma_upd_contains_different_addr h r x r'
+
 
 (* let upd_contains (#a:Type) (#b:Type) (h:heap) (r:ref a) (x:a) (r':ref b) *)
 (*   :Lemma (requires True) *)
@@ -298,19 +269,19 @@ let lemma_upd_unused (#a:Type) (#b:Type) (h:heap) (r:ref a) (x:a) (r':ref b)
   :Lemma (requires True)
          (ensures  ((addr_of r <> addr_of r' /\ r' `unused_in` h) <==> r' `unused_in` (upd h r x)))
 	 [SMTPat (r' `unused_in` (upd h r x))]
-  = ()
+  = lemma_upd_unused h r x r'
 
 let lemma_contains_upd_modifies (#a:Type) (h:heap) (r:ref a) (x:a)
   :Lemma (requires (h `contains` r))
          (ensures  (modifies (Set.singleton (addr_of r)) h (upd h r x)))
          [SMTPat (upd h r x); SMTPat (h `contains` r)]
-  = ()
+  = lemma_contains_upd_modifies h r x
 
 let lemma_unused_upd_modifies (#a:Type) (h:heap) (r:ref a) (x:a)
   :Lemma (requires (r `unused_in` h))
          (ensures  (modifies (Set.singleton (addr_of r)) h (upd h r x)))
          [SMTPat (upd h r x); SMTPat (r `unused_in` h)]
-  = ()
+  = lemma_unused_upd_modifies h r x
 
 (* let lemma_modifies_trans (h1:heap) (h2:heap) (h3:heap) (s1:set nat) (s2:set nat) *)
 (*   :Lemma (requires (modifies s1 h1 h2 /\ modifies s2 h2 h3)) *)
@@ -318,20 +289,18 @@ let lemma_unused_upd_modifies (#a:Type) (h:heap) (r:ref a) (x:a)
 (* 	 [SMTPat (modifies s1 h1 h2); SMTPat (modifies s2 h2 h3)] *)
 (*   = () *)
 
-abstract let equal (h1:heap) (h2:heap) :Type0 =
-  h1.next_addr = h2.next_addr /\
-  FStar.FunctionalExtensionality.feq h1.memory h2.memory
+abstract let equal (h1:heap) (h2:heap) :Type0 = equal h1 h2
 
 val equal_extensional: h1:heap -> h2:heap
                        -> Lemma (requires True) (ensures (equal h1 h2 <==> h1 == h2))
 		         [SMTPat (equal h1 h2)]
-let equal_extensional h1 h2 = ()			 
+let equal_extensional h1 h2 = equal_extensional h1 h2			 
 
 let upd_upd_same_ref (#a:Type) (h:heap) (r:ref a) (x:a) (y:a)
   :Lemma (requires True)
          (ensures  (upd (upd h r x) r y == upd h r y))
 	 [SMTPat (upd (upd h r x) r y)]
-  = assert (equal (upd (upd h r x) r y) (upd h r y))
+  = () //assert (equal (upd (upd h r x) r y) (upd h r y))
 
 val op_Hat_Plus_Plus: #a:Type -> r:ref a -> set nat -> GTot (set nat)
 let op_Hat_Plus_Plus #a r s = union (only r) s
@@ -341,3 +310,16 @@ let op_Plus_Plus_Hat #a s r = union s (only r)
 
 val op_Hat_Plus_Hat: #a:Type -> #b:Type -> ref a -> ref b -> GTot (set nat)
 let op_Hat_Plus_Hat #a #b r1 r2 = union (only r1) (only r2)
+
+
+(* lemmas to pass regressions *)
+
+private let lemma_contains (#a:Type0) (h:heap) (r:ref a)
+  :Lemma (contains h r <==> FStar.Monotonic.Heap.contains h r)
+         [SMTPat (contains h r)]
+  = ()
+
+private let lemma_unused_in (#a:Type0) (r:ref a) (h:heap)
+  :Lemma (unused_in r h <==> FStar.Monotonic.Heap.unused_in r h)
+         [SMTPat (unused_in r h)]
+  = ()
